fix: public accesses to private defs

src/Init/Core.lean
@@ -118,6 +118,10 @@ Computed values are cached, so the value is not recomputed.
 @[extern "lean_thunk_get_own"] protected def Thunk.get (x : @& Thunk α) : α :=
   x.fn ()
 
+-- Ensure `Thunk.fn` is still computable even if it shouldn't be accessed directly.
+@[inline] private def Thunk.fnImpl (x : Thunk α) : Unit → α := fun _ => x.get
+@[csimp] private theorem Thunk.fn_eq_fnImpl : @Thunk.fn = @Thunk.fnImpl := rfl
+
 /--
 Constructs a new thunk that forces `x` and then applies `x` to the result. Upon forcing, the result
 of `f` is cached and the reference to the thunk `x` is dropped.
