src/Init/Meta.lean
@@ -8,6 +8,7 @@ Additional goodies for writing macros
 module
 
 prelude
+import all Init.Prelude  -- for unfolding `Name.beq`
 import Init.MetaTypes
 import Init.Syntax
 import Init.Data.Array.GetLit
@@ -1203,7 +1204,8 @@ def quoteNameMk : Name → Term
   | .num n i => Syntax.mkCApp ``Name.mkNum #[quoteNameMk n, quote i]
 
 instance : Quote Name `term where
-  quote n := match getEscapedNameParts? [] n with
+  quote n := private
+    match getEscapedNameParts? [] n with
     | some ss => ⟨mkNode `Lean.Parser.Term.quotedName #[Syntax.mkNameLit ("`" ++ ".".intercalate ss)]⟩
     | none    => ⟨quoteNameMk n⟩
 
@@ -1216,7 +1218,7 @@ private def quoteList [Quote α `term] : List α → Term
   | (x::xs) => Syntax.mkCApp ``List.cons #[quote x, quoteList xs]
 
 instance [Quote α `term] : Quote (List α) `term where
-  quote := quoteList
+  quote := private quoteList
 
 private def quoteArray [Quote α `term] (xs : Array α) : Term :=
   if xs.size <= 8 then
@@ -1233,7 +1235,7 @@ where
   decreasing_by decreasing_trivial_pre_omega
 
 instance [Quote α `term] : Quote (Array α) `term where
-  quote := quoteArray
+  quote := private quoteArray
 
 instance Option.hasQuote {α : Type} [Quote α `term] : Quote (Option α) `term where
   quote
